Use uint64 in Pos
This affects a lot of code -it effectively maintains an invariant within
a Pos that's independent of the config. However Pos is used at runtime
to compute inode and indirect block offsets so it's a big win to avoid
all of this use of big nums. It's really annoying to do this "properly"
with separate specification and runtime types and relations between
them, so we just fix the spec type to build in this stronger invariant.

src/Dafny/examples/fs/block_fs.dfy
@@ -28,13 +28,13 @@ module BlockFs
     requires data_dom(data)
   {
     var blks := seq(config.total,
-      (n:nat) requires n < config.total => data[Pos.from_flat(ino, n)]);
+      (n:nat) requires n < config.total => data[Pos.from_flat(ino, n as uint64)]);
     InodeData(blks)
   }
 
-  predicate is_lba(i: int)
+  predicate is_lba(i: uint64)
   {
-    0 <= i < config.total
+    i as nat < config.total
   }
 
   function {:opaque} block_data(data: imap<Pos, Block>): (m:map<Ino, InodeData>)
@@ -58,7 +58,7 @@ module BlockFs
   }
 
   // public
-  method Read<InodeAllocState(!new)>(fs: IndFilesys<InodeAllocState>, txn: Txn, ino: Ino, i: Inode.Inode, n: nat)
+  method Read<InodeAllocState(!new)>(fs: IndFilesys<InodeAllocState>, txn: Txn, ino: Ino, i: Inode.Inode, n: uint64)
     returns (bs: Bytes)
     requires fs.ValidIno(ino, i)
     requires fs.has_jrnl(txn)
@@ -78,7 +78,7 @@ module BlockFs
     ensures m2 == m1[k0 := v]
   {}
 
-  lemma block_data_update(data: imap<Pos, Block>, ino: Ino, n: nat, blk: Block)
+  lemma block_data_update(data: imap<Pos, Block>, ino: Ino, n: uint64, blk: Block)
     requires is_lba(n)
     requires data_dom(data)
     ensures inode_blocks(ino, data[Pos.from_flat(ino, n) := blk]).blks ==
@@ -103,7 +103,7 @@ module BlockFs
   }
 
   // an update to an ino0 Pos doesn't affect ino
-  lemma block_data_update_other(data: imap<Pos, Block>, ino0: Ino, ino: Ino, n: nat, blk: Block)
+  lemma block_data_update_other(data: imap<Pos, Block>, ino0: Ino, ino: Ino, n: uint64, blk: Block)
     requires is_lba(n)
     requires ino != ino0
     requires data_dom(data)
@@ -124,7 +124,7 @@ module BlockFs
   }
 
   // public
-  method Do(txn: Txn, ino: Ino, i: Inode.Inode, n: nat, blk: Bytes)
+  method Do(txn: Txn, ino: Ino, i: Inode.Inode, n: uint64, blk: Bytes)
     returns (ok: bool, i': Inode.Inode)
     modifies fs.Repr
     requires fs.ValidIno(ino, i) ensures fs.ValidIno(ino, i')
@@ -177,18 +177,18 @@ module BlockFs
               C.splice(s, start, C.repeat(x, count))[start + count := x]
     {}
 
-    method Do(txn: Txn, ghost ino: Ino, i: Inode.Inode, start: nat, len: nat)
+    method Do(txn: Txn, ghost ino: Ino, i: Inode.Inode, start: uint64, len: uint64)
       returns (i': Inode.Inode)
       modifies fs.Repr
       requires fs.ValidIno(ino, i) ensures fs.ValidIno(ino, i')
       requires fs.has_jrnl(txn)
       //requires start + len <= config.total
-      requires start + len <= 10
+      requires start as nat + len as nat <= 10
       ensures block_data(fs.data) ==
       (var data := old(block_data(fs.data));
       var d0 := data[ino];
       var blks0 := d0.blks;
-      var blks' := C.splice(blks0, start, C.repeat(block0, len));
+      var blks' := C.splice(blks0, start as nat, C.repeat(block0, len as nat));
       data[ino := d0.(blks := blks')]
       )
       ensures fs.metadata == old(fs.metadata)
@@ -198,13 +198,14 @@ module BlockFs
       ghost var d0 := data0[ino];
       ghost var blks0 := d0.blks;
       assert C.repeat(block0, 0) == [];
-      assert C.splice(blks0, start, []) == blks0;
-      var k := 0;
+      assert C.splice(blks0, start as nat, []) == blks0;
+      var k: uint64 := 0;
       while k < len
         modifies fs.Repr
         invariant 0 <= k <= len
         invariant fs.ValidIno(ino, i')
-        invariant block_data(fs.data)[ino].blks == C.splice(blks0, start, C.repeat(block0, k))
+        invariant block_data(fs.data)[ino].blks ==
+                  C.splice(blks0, start as nat, C.repeat(block0, k as nat))
         invariant forall ino': Ino | ino' != ino ::
           block_data(fs.data)[ino'] == old(block_data(fs.data)[ino'])
         invariant fs.metadata == old(fs.metadata)
@@ -219,7 +220,7 @@ module BlockFs
           reveal block_data();
           block_data_update(fsdata_prev, ino, n, block0);
         }
-        splice_repeat_one_more(blks0, start, k, block0);
+        splice_repeat_one_more(blks0, start as nat, k as nat, block0);
 
         forall ino':Ino | ino' != ino
           ensures block_data(fs.data)[ino'] == old(block_data(fsdata_prev)[ino'])
