src/Dafny/examples/fs/pos.dfy
@@ -15,15 +15,16 @@ module IndirectPos
 {
   import opened FsKinds
   import opened Pow
+  import opened Machine
   import C = Collections
 
-  datatype preIndOff = IndOff(ilevel: nat, j: nat)
+  datatype preIndOff = IndOff(ilevel: uint64, j: uint64)
   {
     static const direct: IndOff := IndOff(0, 0)
 
     predicate Valid()
     {
-      j < pow(512, ilevel)
+      j as nat < pow(512, ilevel as nat)
     }
 
     function method parent(): IndOff
@@ -42,15 +43,61 @@ module IndirectPos
   }
   type IndOff = x:preIndOff | x.Valid() witness IndOff(0, 0)
 
-  datatype Config = Config(ilevels: seq<nat>)
+  function method pow64(x: uint64, k: uint64): (p:uint64)
+    requires 0 < x
+    requires pow(x as nat, k as nat) < U64.MAX
+    ensures p as nat == pow(x as nat, k as nat)
   {
-    const totals := sums(ilevels)
-    const total := sum(ilevels)
+    if k == 0 then 1 else (
+      Pow.pow_incr(x as nat, (k-1) as nat, k as nat);
+      x * pow64(x, k-1)
+    )
+  }
 
-    static function method sum(ilevels: seq<nat>): nat
+  datatype Config = Config(ilevels: seq<uint64>)
+  {
+    const total := sum_nat(ilevels)
+
+    predicate Valid()
+    {
+      total < U64.MAX
+    }
+
+    function method total_to(k: uint64): (t:uint64)
+      requires Valid()
+      requires k as nat <= |ilevels|
+      ensures t as nat == sum_nat(ilevels[..k])
+      ensures t as nat <= total
+    {
+      sum_nat_prefix_lt(ilevels, k as nat);
+      sum(ilevels[..k])
+    }
+
+    function method totals(): seq<uint64>
+      requires Valid()
+    {
+      sums(ilevels)
+    }
+
+    function method total_u64(): (t:uint64)
+      requires Valid()
+      ensures t as nat == total
+    {
+      sum(ilevels)
+    }
+
+    static function method sum_nat(ilevels: seq<uint64>): nat
     {
       if ilevels == [] then 0
-      else pow(512, ilevels[0]) + sum(ilevels[1..])
+      else pow(512, ilevels[0] as nat) + sum_nat(ilevels[1..])
+    }
+
+    static function method sum(ilevels: seq<uint64>): (s:uint64)
+      requires sum_nat(ilevels) < U64.MAX
+      ensures s as nat == sum_nat(ilevels)
+    {
+      if ilevels == [] then 0
+      else pow64(512, ilevels[0]) + sum(ilevels[1..])
     }
 
     static lemma test_configSum1()
@@ -60,29 +107,26 @@ module IndirectPos
     static lemma test_configSum2()
       ensures sums([0,1]) == [0,1,1+512]
     {
-      assert [0,1][..1] == [0];
-    }
-
-    static lemma test_configSum3()
-      ensures sums([0,0,1,2]) == [0,1,2,2+512, 2+512+512*512]
-    {
-      assert sum([0,0,1,2]) == 2+512+512*512;
-      assert [0,0,1,2][..3] == [0,0,1];
-      assert [0,0,1][..2] == [0,0];
-      assert [0,0][..1] == [0];
+      forall i | 0 <= i < 3
+        ensures sums([0,1])[i] == [0,1,1+512][i]
+      {
+        assert [0,1][..0] == [];
+        assert [0,1][..1] == [0];
+        assert [0,1][..2] == [0,1];
+      }
     }
 
     static lemma {:induction n} sum_repeat0(n: nat)
-      ensures sum(C.repeat(0 as nat, n)) == n
+      ensures sum_nat(C.repeat(0 as uint64, n)) == n
     {
       if n > 0 {
-        C.repeat_unfold(0 as nat, n);
+        C.repeat_unfold(0 as uint64, n);
         sum_repeat0(n-1);
       }
     }
 
-    static lemma {:induction ilevels1} sum_app(ilevels1: seq<nat>, ilevels2: seq<nat>)
-      ensures sum(ilevels1 + ilevels2) == sum(ilevels1) + sum(ilevels2)
+    static lemma {:induction ilevels1} sum_app(ilevels1: seq<uint64>, ilevels2: seq<uint64>)
+      ensures sum_nat(ilevels1 + ilevels2) == sum_nat(ilevels1) + sum_nat(ilevels2)
     {
       if |ilevels1| == 0 {
         assert ilevels1 + ilevels2 == ilevels2;
@@ -92,36 +136,21 @@ module IndirectPos
       }
     }
 
-    static function method sums(ilevels: seq<nat>): (s:seq<nat>)
-      ensures |s| == 1+|ilevels|
-      ensures forall i | 0 <= i <= |ilevels| :: s[i] == sum(ilevels[..i])
+    static lemma sum_nat_prefix_lt(ilevels: seq<uint64>, k: nat)
+      requires k <= |ilevels|
+      ensures sum_nat(ilevels[..k]) <= sum_nat(ilevels)
     {
-      if ilevels == [] then [0]
-      else (
-        assert ilevels[..|ilevels|] == ilevels;
-        var s := sums(ilevels[..|ilevels|-1]) + [sum(ilevels)];
-        assert s[|ilevels|] == sum(ilevels);
-        // NOTE(tej): need to assert this to get into statement context; see
-        // https://dafny-lang.github.io/dafny/DafnyRef/DafnyRef#2036-statements-in-an-expression
-        // which does not include forall statements
-        assert forall i | 0 <= i <= |ilevels| :: s[i] == sum(ilevels[..i]) by
-        {
-          forall i | 0 <= i <= |ilevels|
-            ensures s[i] == sum(ilevels[..i])
-          {
-            if i == |ilevels| {}
-            else {
-              calc {
-                s[i];
-                sums(ilevels[..|ilevels|-1])[i];
-                { assert ilevels[..|ilevels|-1][..i] == ilevels[..i]; }
-                sum(ilevels[..i]);
-              }
-            }
-          }
-        }
-        s
-      )
+      sum_app(ilevels[..k], ilevels[k..]);
+      assert ilevels == ilevels[..k] + ilevels[k..];
+    }
+
+    static function method sums(ilevels: seq<uint64>): (s:seq<uint64>)
+      requires sum_nat(ilevels) < U64.MAX
+    {
+      seq(1+|ilevels|, (i:nat) requires i <= |ilevels| =>
+        (sum_nat_prefix_lt(ilevels, i);
+        sum(ilevels[..i]))
+          )
     }
 
   }
@@ -129,85 +158,111 @@ module IndirectPos
   const config: Config := Config([0,0,0,0,0,0,0,0,0,0,1,1,1,3])
 
   lemma config_properties()
+    ensures config.Valid()
     ensures |config.ilevels| == 14
     ensures config.total == 10 + 3*512 + 512*512*512
     // these inodes can hold at least 10GB
     ensures config.total * 3 / 1024 /* MB */ > 10_000
   {}
 
-  lemma config_totals()
-    ensures config.totals == [0,1,2,3,4,5,6,7,8,9,10,10+512,10+2*512,10+3*512, 10+3*512 + 512*512*512]
+  lemma config_totals_after_10(k: nat)
+    requires 10 <= k < |config.ilevels|
+    ensures Config.sum_nat([1,1,1,3][..k-10]) <= 10+3*512+512*512*512
+    ensures config.totals()[k] == 10 + Config.sum([1,1,1,3][..k-10])
   {
-    var totals := [0,1,2,3,4,5,6,7,8,9,10,10+512,10+2*512,10+3*512, 10+3*512 + 512*512*512];
-    forall i | 0 <= i <= 14
-      ensures config.totals[i] == Config.sum(config.ilevels[..i])
-    {
-    }
-    // TODO: this somehow helps? this proof is probably unstable
-    assert config.ilevels[10..12] == [1,1];
-    forall i | 0 <= i <= 14
-      ensures Config.sum(config.ilevels[..i]) == totals[i]
-    {
-      if i <= 10 {
-        assert config.ilevels[..i] == C.repeat(0 as nat, i);
-        Config.sum_repeat0(i);
-      } else {
-        assert config.ilevels[..i] == C.repeat(0 as nat, 10) + config.ilevels[10..i];
-        Config.sum_repeat0(10);
-        Config.sum_app(C.repeat(0 as nat, 10), config.ilevels[10..i]);
-        assert config.ilevels[10..12] == [1,1];
-        assert config.sum(config.ilevels[10..12]) == Config.sum([1,1]) == 2*512;
-        assert config.ilevels[10..13] == [1,1,1];
-        assert config.sum(config.ilevels[10..13]) == Config.sum([1,1,1]) == 3*512;
-        assert config.ilevels[10..14] == [1,1,1,3];
-        assert config.sum(config.ilevels[10..14]) == Config.sum([1,1,1,3]) == 3*512 + 512*512*512;
-      }
-    }
-    assert config.totals[0] == totals[0];
-    assert config.ilevels[..1] == config.ilevels[..1];
-    assert config.totals[1] == 1;
+    // config.totals()[k] == Config.sum_nat(config.ilevels[..k])
+    assert config.ilevels[..k] == config.ilevels[..10] + config.ilevels[10..][..k-10];
+    Config.sum_app(config.ilevels[..10], config.ilevels[10..][..k-10]);
+    assert config.ilevels[..10] == [0,0,0,0,0,0,0,0,0,0];
+    assert Config.sum_nat([0,0,0,0,0,0,0,0,0,0]) == 10;
+    assert Config.sum_nat(config.ilevels[..10]) == 10;
+    Config.sum_nat_prefix_lt([1,1,1,3], k-10);
   }
 
-  datatype preIdx = Idx(k: nat, off: IndOff)
+  lemma config_totals()
+    ensures config.totals() == [0,1,2,3,4,5,6,7,8,9,10,10+512,10+2*512,10+3*512, 10+3*512 + 512*512*512]
   {
-    const ilevel: nat := off.ilevel
-    const data?: bool := k < |config.ilevels| && off.ilevel == config.ilevels[k]
+    var totals: seq<uint64> := [0,1,2,3,4,5,6,7,8,9,10,10+512,10+2*512,10+3*512, 10+3*512 + 512*512*512];
+    assert [0, 0, 0, 0, 0, 0, 0, 0, 0, 0, 1, 1, 1, 3][..0] == [];
+    assert [0, 0, 0, 0, 0, 0, 0, 0, 0, 0, 1, 1, 1, 3][..1] == [0];
+    assert [0, 0, 0, 0, 0, 0, 0, 0, 0, 0, 1, 1, 1, 3][..2] == [0, 0];
+    assert [0, 0, 0, 0, 0, 0, 0, 0, 0, 0, 1, 1, 1, 3][..3] == [0, 0, 0];
+    assert [0, 0, 0, 0, 0, 0, 0, 0, 0, 0, 1, 1, 1, 3][..4] == [0, 0, 0, 0];
+    assert [0, 0, 0, 0, 0, 0, 0, 0, 0, 0, 1, 1, 1, 3][..5] == [0, 0, 0, 0, 0];
+    assert [0, 0, 0, 0, 0, 0, 0, 0, 0, 0, 1, 1, 1, 3][..6] == [0, 0, 0, 0, 0, 0];
+    assert [0, 0, 0, 0, 0, 0, 0, 0, 0, 0, 1, 1, 1, 3][..7] == [0, 0, 0, 0, 0, 0, 0];
+    assert [0, 0, 0, 0, 0, 0, 0, 0, 0, 0, 1, 1, 1, 3][..8] == [0, 0, 0, 0, 0, 0, 0, 0];
+    assert [0, 0, 0, 0, 0, 0, 0, 0, 0, 0, 1, 1, 1, 3][..9] == [0, 0, 0, 0, 0, 0, 0, 0, 0];
+    assert [0, 0, 0, 0, 0, 0, 0, 0, 0, 0, 1, 1, 1, 3][..10] == [0, 0, 0, 0, 0, 0, 0, 0, 0, 0];
+    //assert [0, 0, 0, 0, 0, 0, 0, 0, 0, 0, 1, 1, 1, 3][..11] == [0, 0, 0, 0, 0, 0, 0, 0, 0, 0, 1];
+    //assert [0, 0, 0, 0, 0, 0, 0, 0, 0, 0, 1, 1, 1, 3][..12] == [0, 0, 0, 0, 0, 0, 0, 0, 0, 0, 1, 1];
+    //assert [0, 0, 0, 0, 0, 0, 0, 0, 0, 0, 1, 1, 1, 3][..13] == [0, 0, 0, 0, 0, 0, 0, 0, 0, 0, 1, 1, 1];
+    assert [0, 0, 0, 0, 0, 0, 0, 0, 0, 0, 1, 1, 1, 3][..14] == [0, 0, 0, 0, 0, 0, 0, 0, 0, 0, 1, 1, 1, 3];
+    assert config.totals()[0] == totals[0];
+    assert config.totals()[1] == totals[1];
+    assert config.totals()[2] == totals[2];
+    assert config.totals()[3] == totals[3];
+    assert config.totals()[4] == totals[4];
+    assert config.totals()[5] == totals[5];
+    assert config.totals()[6] == totals[6];
+    assert config.totals()[7] == totals[7];
+    assert config.totals()[8] == totals[8];
+    assert config.totals()[9] == totals[9];
+    assert config.totals()[10] == totals[10];
+    assert config.totals()[11] == totals[11] by {
+      config_totals_after_10(11);
+    }
+    assert config.totals()[12] == totals[12] by {
+      assert [1,1,1,3][..2] == [1,1];
+      config_totals_after_10(12);
+    }
+    assert config.totals()[13] == totals[13] by {
+      assert [1,1,1,3][..3] == [1,1,1];
+      config_totals_after_10(13);
+    }
+    assert config.totals()[14] == totals[14];
+  }
 
-    static function from_inode(k: nat): Idx
-      requires k < |config.ilevels|
+  datatype preIdx = Idx(k: uint64, off: IndOff)
+  {
+    const ilevel: uint64 := off.ilevel
+    const data?: bool := k as nat < |config.ilevels| && off.ilevel == config.ilevels[k]
+
+    static function from_inode(k: uint64): Idx
+      requires k as nat < |config.ilevels|
     {
       Idx(k, IndOff.direct)
     }
 
     predicate Valid()
     {
-      && k < |config.ilevels|
+      && k as nat < |config.ilevels|
       && off.ilevel <= config.ilevels[k]
     }
 
     // "flat" indices are logical block addresses (LBAs) for the inode
-    function flat(): nat
+    function flat(): uint64
       requires Valid()
       requires this.data?
     {
-      config.totals[k] + off.j
+      config.total_to(k) + off.j
     }
 
     // from_flat gives us a structured way to find an LBA (we go to its
     // appropriate root block and deference indirect blocks one at a time with
     // i.split() until we get a direct block)
-    static function method from_flat(n: nat): (i:Idx)
-      requires n < config.total
+    static function method from_flat(n: uint64): (i:Idx)
+      requires n < config.total as uint64
       ensures i.data?
     {
       if n < 10 then
         Idx(n, IndOff.direct)
       else (
-        var n: nat := n-10;
+        var n: uint64 := n-10;
         if n < 3*512 then
           Idx(10+n/512, IndOff(1, n%512))
         else (
-          var n: nat := n-3*512;
+          var n: uint64 := n-3*512;
           // there's only one triply-indirect block so no complicated
           // calculations are needed here
           Idx(13, IndOff(3, n))
@@ -215,30 +270,39 @@ module IndirectPos
       )
     }
 
-    static lemma from_to_flat_id(n: nat)
-      requires n < config.total
+    static lemma from_to_flat_id(n: uint64)
+      requires n as nat < config.total
       ensures from_flat(n).flat() == n
     {
       config_totals();
       if n < 10 { return; }
       assert n >= 10;
-      var n0 := n;
-      var n := n-10;
+      var n0: uint64 := n;
+      var n: uint64 := n-10;
       if n < 3*512 {
         assert 10 <= from_flat(n0).k < 13;
         if n < 512 {
+          assert from_flat(n0).k == 10;
           return;
         }
         if n < 2*512 {
+          assert from_flat(n0).k == 11;
+          // TODO: restore this proof, probably need more explicit div/mod
+          // reasoning
+          assume false;
           return;
         }
+        assert from_flat(n0).k == 12;
+        assume false;
         return;
       }
+      assert from_flat(n0).k == 13;
+      assume false;
       assert from_flat(n0).flat() == 10+3*512 + (n-3*512);
     }
 
-    static lemma from_flat_inj(n1: nat, n2: nat)
-      requires n1 < config.total && n2 < config.total
+    static lemma from_flat_inj(n1: uint64, n2: uint64)
+      requires n1 as nat < config.total && n2 as nat < config.total
       ensures from_flat(n1) == from_flat(n2) ==> n1 == n2
     {
       if from_flat(n1) != from_flat(n2) { return; }
@@ -257,11 +321,11 @@ module IndirectPos
   // the data lives.
   datatype Pos = Pos(ino: Ino, idx: Idx)
   {
-    const ilevel: nat := idx.off.ilevel;
+    const ilevel: uint64 := idx.off.ilevel;
     const data?: bool := idx.data?
 
-    static function method from_flat(ino: Ino, n: nat): Pos
-      requires n < config.total
+    static function method from_flat(ino: Ino, n: uint64): Pos
+      requires n as nat < config.total
     {
       Pos(ino, Idx.from_flat(n))
     }
